Adding bank account with superglobal invariant + mutable linked list

Test/uncooperativeconcurrency/concurrenthashmap.dfy
@@ -37,6 +37,16 @@ class Entry<K(==), V> {
          && next in Repr
          && next.Invariant()
   }
+  twostate lemma InvariantDoesNotDependOnValue()
+    requires old(Invariant())
+    requires forall e <- Repr | (e is Entry<K, V>) :: e.next == old(e.next)
+    ensures Invariant()
+    decreases |Repr|
+  {
+    if next != null {
+      next.InvariantDoesNotDependOnValue();
+    }
+  }
 
   // Ensures that the first entries override the last ones
   ghost function ToModel(): map<K, V> reads this, Repr
@@ -72,30 +82,23 @@ class ConcurrentHashMap<K(==), V> {
     var entry := entries[startIndex];
     rec + (if entry == null then map[] else entries[startIndex].ToModel())
   }
-  ghost predicate InvariantPerEntry2(i: int)
-    reads this, entries, segments, Repr
-    requires entries.Length == segments.Length
-    requires 0 <= i < segments.Length
-    requires InvariantPerEntry(entries[i])
-  {
-    segments[i] in Repr &&
-    if entries[i] != null then
-      && segments !in entries[i].Repr
-      && segments[i].count == entries[i].Count()
-    else
-      && segments[i].count == 0
-  }
-  ghost predicate InvariantPerEntry(entry: Entry?<K, V>)
+  ghost predicate InvariantPerEntry0(entry: Entry?<K, V>)
     reads this
     reads entry
-    reads if entry != null then entry.Repr else {}
   {
     entry != null ==>
-      && this !in entry.Repr
-      && entries !in entry.Repr
       && entry in Repr
       && entry.Repr <= Repr
-      && entry.Invariant()
+      && this !in entry.Repr
+      && entries !in entry.Repr
+  }
+  ghost predicate InvariantPerEntry1(entry: Entry?<K, V>)
+    reads this
+    reads entry
+          reads if entry != null then entry.Repr else {}
+    requires InvariantPerEntry0(entry)
+  {
+    entry != null ==> entry.Invariant()
   }
   ghost predicate Invariant()
     reads this, Repr
@@ -106,11 +109,28 @@ class ConcurrentHashMap<K(==), V> {
     && entries.Length == segments.Length
     && entries.Length >= 1
     && (forall i: nat | 0 <= i < this.entries.Length ::
-          (entries[i] != null ==> entries[i] in Repr && entries[i].Repr <= Repr) &&
-          InvariantPerEntry(entries[i]) && InvariantPerEntry2(i))
+          && (entries[i] != null ==> entries[i] in Repr)
+          && InvariantPerEntry0(entries[i])
+          && InvariantPerEntry1(entries[i])
+          && InvariantPerEntry2(i))
     && (forall i: nat, j: nat | i < entries.Length && j < entries.Length && i != j ::
           entries[i] == null || entries[j] == null ||
           entries[i].Repr !! entries[j].Repr)
+  }
+  ghost predicate InvariantPerEntry2(i: int)
+    reads this, entries, segments, Repr
+    requires entries.Length == segments.Length
+    requires 0 <= i < segments.Length
+    requires InvariantPerEntry0(entries[i])
+    requires InvariantPerEntry1(entries[i])
+  {
+    segments[i] in Repr &&
+    if entries[i] != null then
+      && segments !in entries[i].Repr
+      && segments[i].count == entries[i].Count()
+      && (forall j | 0 <= j < segments.Length :: segments[j] !in entries[i].Repr)
+    else
+      && segments[i].count == 0
   }
 
   function Hash(k: K): int // Needs to be given!
@@ -123,7 +143,7 @@ class ConcurrentHashMap<K(==), V> {
       var hash := Hash(k);
       var indexEntry := hash % entries.Length;
       var e := entries[indexEntry];
-      assert InvariantPerEntry(entries[indexEntry]);
+      assert InvariantPerEntry1(entries[indexEntry]);
       assert e != null ==> e in Repr;
       while(e != null)
         invariant Invariant()
@@ -133,8 +153,18 @@ class ConcurrentHashMap<K(==), V> {
         if e.hash == hash && k == e.key { // if key already exist means updating the value
           var oldValue := e.value;
           assert Invariant();
+          label before:
           e.value := v;
-          assert Invariant();
+          assert Invariant() by {
+            e.InvariantDoesNotDependOnValue@before();
+            forall i: nat | 0 <= i < this.entries.Length ensures
+                && (entries[i] != null ==> entries[i] in Repr)
+                && InvariantPerEntry0(entries[i])
+                && InvariantPerEntry1(entries[i])
+                && InvariantPerEntry2(i) {
+
+            }
+          }
           return oldValue;
         }
         e := e.next;
@@ -145,23 +175,22 @@ class ConcurrentHashMap<K(==), V> {
       Repr := {newEntry} + Repr;
       assert newEntry.next != null ==> newEntry.next.Invariant();
       assert /*{:only} */&& newEntry in Repr
-                     && newEntry.Repr <= Repr
-                     && newEntry.Invariant();
+                         && newEntry.Repr <= Repr
+                         && newEntry.Invariant();
       assert this as object != entries as object;
       assert this as object != segments as object;
       entries[indexEntry] := newEntry;
       segments[indexEntry].count := segments[indexEntry].count + 1;
-      assert {:only} Invariant() by {
-        assert forall i: nat | 0 <= i < this.entries.Length ::
-            InvariantPerEntry(entries[i]) by {
-          forall i: nat | 0 <= i < this.entries.Length ensures
-              InvariantPerEntry(entries[i]) {
-            if i == indexEntry {
-              assert InvariantPerEntry(entries[i]);
-            } else {
-              assert{:only} InvariantPerEntry(entries[i]) by {
 
-              }
+      assert Invariant() by {
+        assert forall i: nat | 0 <= i < this.entries.Length ::
+            InvariantPerEntry1(entries[i]) by {
+          forall i: nat | 0 <= i < this.entries.Length ensures
+              InvariantPerEntry1(entries[i]) {
+            if i == indexEntry {
+              assert InvariantPerEntry1(entries[i]);
+            } else {
+              assert InvariantPerEntry1(entries[i]);
             }
           }
         }
