Test/uncooperativeconcurrency/BankAccounts.dfy
@@ -1,0 +1,171 @@
+
+// Separated class
+class Account {
+  var money: int
+  method Add(extra: int)
+    modifies this
+    ensures money == old(money) + extra
+  {
+    this.money := this.money + extra;
+  }
+}
+
+// This function requires the caller to have exclusive read access over all the accounts
+function Sum(s: seq<Account>): int reads s {
+  if |s| == 0 then 0 else Sum(s[0..|s|-1]) + s[|s|-1].money
+}
+
+predicate readLocked(s: seq<Account>, extraRights: set<object>) {
+  (set x | x in s) <= extraRights
+}
+
+// Separated but invariant is True.
+class BankAccount {
+  const accounts: seq<Account>
+  var total: int
+
+  predicate Invariant() {
+    forall i, j | 0 <= i < j < |accounts| :: accounts[i] != accounts[j]
+  }
+
+  // Requires to hav exclusive read access over all the accounts, which is not granted usually.
+  predicate GlobalInvariant() reads this, this.accounts {
+    Sum(accounts[..]) == total
+  }
+
+  twostate lemma GlobalInvariantInvariant0(accounts: seq<Account>)
+    requires forall k | 0 <= k < |accounts| :: accounts[k].money == old(accounts[k].money)
+    ensures Sum(accounts[..]) == old(Sum(accounts[..]))
+  {
+    if |accounts| == 0 {
+    } else {
+      calc {
+        Sum(accounts[..]);
+        Sum(accounts[0..|accounts|-1]) + accounts[|accounts|-1].money;
+        Sum(accounts[0..|accounts|-1]) + old(accounts[|accounts|-1].money);
+        { GlobalInvariantInvariant0(accounts[0..|accounts|-1]); }
+        old(Sum(accounts[0..|accounts|-1])) + old(accounts[|accounts|-1].money);
+      }
+    }
+  }
+
+  twostate lemma GlobalInvariantInvariant1(accounts: seq<Account>, i: int, money: int)
+    requires 0 <= i < |accounts|
+    requires accounts[i].money == old(accounts[i].money) + money
+    requires forall k | 0 <= k < |accounts| && k != i :: accounts[k].money == old(accounts[k].money)
+    ensures Sum(accounts[..]) == old(Sum(accounts[..])) + money
+  {
+    if i == |accounts|-1 {
+      calc {
+        Sum(accounts[..]);
+        Sum(accounts[0..|accounts|-1]) + accounts[i].money;
+        Sum(accounts[0..|accounts|-1]) + old(accounts[i].money) + money;
+        { GlobalInvariantInvariant0(accounts[0..|accounts|-1]); }
+        old(Sum(accounts[0..|accounts|-1])) + old(accounts[i].money) + money;
+        old(Sum(accounts[0..|accounts|-1]) + accounts[i].money) + money;
+        old(Sum(accounts[..])) + money;
+      }
+    } else {
+      calc {
+        Sum(accounts[..]);
+        Sum(accounts[0..|accounts|-1]) + accounts[|accounts|-1].money;
+        Sum(accounts[0..|accounts|-1]) + old(accounts[|accounts|-1].money);
+        { GlobalInvariantInvariant1(accounts[0..|accounts|-1], i, money); }
+        (old(Sum(accounts[0..|accounts|-1])) + money) + old(accounts[|accounts|-1].money);
+        old(Sum(accounts[0..|accounts|-1])) + old(accounts[|accounts|-1].money) + money;
+        old(Sum(accounts[0..|accounts|-1]) + accounts[|accounts|-1].money) + money;
+        old(Sum(accounts[..])) + money;
+      }
+    }
+  }
+
+  twostate lemma GlobalInvariantInvariant2(accounts: seq<Account>, i: int, j: int, money: int)
+    requires 0 <= i < j < |accounts|
+    requires accounts[i].money == old(accounts[i].money) + money
+    requires accounts[j].money == old(accounts[j].money) - money
+    requires forall k | 0 <= k < |accounts| && k != i && k != j :: accounts[k].money == old(accounts[k].money)
+    ensures Sum(accounts[..]) == old(Sum(accounts[..]))
+  {
+    if j == |accounts| - 1 {
+      calc {
+        Sum(accounts[..]);
+        Sum(accounts[..j]) + accounts[j].money;
+        { GlobalInvariantInvariant1(accounts[..j], i, money); }
+        (old(Sum(accounts[..j])) + money) + accounts[j].money;
+        (old(Sum(accounts[..j])) + money) + (old(accounts[j].money) - money);
+        old(Sum(accounts[..j])) + old(accounts[j].money);
+        old(Sum(accounts[..]));
+      }
+    } else {
+      calc {
+        Sum(accounts[..]);
+        { GlobalInvariantInvariant2(accounts[..|accounts|-1], i, j, money); }
+        old(Sum(accounts[..]));
+      }
+    }
+  }
+
+  // extraRights encode the fact that we could access the frame condition using a predicate
+  // so that there might be objects at the beginning we had the right to modify
+  // At the call site, if these objects are in the modifies clause, then the postcondition holds
+  method Transfer(i: int, money: int, j: int, extraRights: set<object>)
+    requires Invariant()
+    modifies this, extraRights, if 0 <= i < |accounts| && 0 <= j < |accounts| && i != j then
+       {accounts[i] as object, accounts[j]} else {}
+    ensures Invariant()
+    ensures readLocked(this.accounts, extraRights) && old(GlobalInvariant()) ==> GlobalInvariant()
+  {
+    if 0 <= i < |accounts| && 0 <= j < |accounts| && i != j {
+      accounts[i].Add(money);
+      accounts[j].Add(-money);
+      if i < j {
+        GlobalInvariantInvariant2(accounts, i, j, money);
+      } else {
+        assert j < i;
+        GlobalInvariantInvariant2(accounts, j, i, -money);
+      }
+      assert readLocked(this.accounts, extraRights) && old(GlobalInvariant()) ==> GlobalInvariant();
+    } else {
+      assert readLocked(this.accounts, extraRights) && old(GlobalInvariant()) ==> GlobalInvariant();
+    }
+  }
+}
+
+/*method Test(separatedClass: SeparatedClass)
+  modifies separatedClass                     // Usually not needed, since the lock is auto-acquired!
+  modifies separatedClass.OtherSeparatedClass // Even less needed... but this guarantees sequentiality
+  requires separatedClass.Invariant()
+  requires separatedClass.otherSeparatedClass.Invariant()
+{
+  // Still not possible to modify fields directly because of the region rule.
+  separatedClass.Add(1); // Here the region is different, the invariant is assumed.
+  separatedClass.Add(2);
+}*/
+
+
+
+
+
+
+
+
+
+
+
+
+
+
+
+
+
+
+
+
+
+
+
+
+
+
+
+
