Test/uncooperativeconcurrency/concurrentmutablelinkedlist.dfy
@@ -1,0 +1,244 @@
+trait HasOwner {
+  ghost const owner: object?
+
+  // Axiom in boogie that states that
+  // modifylocked(this.owner) ==> modifyLocked(this)
+  // readLocked(this.owner) ==> readLocked(this)
+}
+
+method Test<A>(m: MutableLinkedList<A>, a: A)
+  modifies m, m.Repr // assumed at call site if class is separated
+  requires m.Valid() // assumed at call site if class is separated
+{
+  m.insertElemAt(0, a);
+}
+
+class MutableLinkedList<A>
+  extends HasOwner              // OWNER:
+{
+  var head: Node?<A>
+  ghost var Repr: set<object>
+  var size: int
+  constructor(ghost owner: object?)
+  ensures Valid()
+    ensures this.owner == owner
+  {
+    head := null;
+    Repr := {this};
+    size := 0;
+    this.owner := owner;
+  }
+  ghost predicate Valid()
+    reads this, Repr  
+  {
+    && this in Repr
+    && (forall t: HasOwner :: t in {this} + Repr ==> t == this || t.owner == this)
+    && ((head == null && size == 0) ||
+        ( && head in Repr
+          && head.owner == this             // OWNER:
+          && head.Repr == Repr - {this}
+          && head.size == size
+          && head.Valid()))
+  }
+
+  function elemAt(index: nat): A
+    reads this, Repr
+    requires Valid()
+    requires index < size
+  {
+    // OWNER(auto):
+    assert head.owner == this ||
+      (if this.owner != null then head as object == this else head.owner == null);
+    head.elemAt(index)
+  }
+
+   method replaceElemAt(index: nat, newElem: A)
+    modifies Repr
+    requires Valid()
+    ensures Repr == old(Repr)
+    ensures Valid()
+    requires index < size
+  {
+    assert head.owner == this ||
+      (if this.owner != null then head as object == this else head.owner == null);              // OWNER (auto):
+    head.replaceElemAt(index, newElem);
+  }
+
+  method insertElemAt(index: nat, newElem: A)
+    requires Valid()
+    requires index <= size // Need to be waited for
+    modifies Repr
+    ensures Valid()
+    ensures size == old(size) + 1
+  {
+    if head == null {
+      head := new Node<A>(this, newElem, null);
+      size := 1;
+    } else {
+      ghost var dummy;
+      assert head.owner == this ||
+      (if this.owner != null then head as object == this else head.owner == null);      // OWNER (auto): 
+      head, dummy := head.insertElemAt(index, newElem);
+      size := size + 1;
+    }
+    Repr := {this} + head.Repr;
+  }
+
+  method deleteElemAt(index: nat) returns (a: A)
+    requires Valid()      // Can be assumed only if trying to acquire a lock
+    requires index < size // Need to be waited for and tested
+    modifies Repr
+    ensures Valid()
+    ensures size == old(size) - 1 // Useless at call site unless lock was acquire before
+    ensures a == old(elemAt(index))
+  {
+    assert head.owner == this ||
+      (if this.owner != null then head as object == this else head.owner == null);     // OWNER (auto): 
+    head, a := head.deleteElemAt(index);
+    size := size - 1;
+    Repr := if head == null then {this} else {this} + head.Repr;
+  }
+}
+
+class Node<A> extends HasOwner {
+  var value: A
+  var next: Node?<A>
+  var size: nat
+  ghost var Repr: set<object>
+
+  constructor(ghost owner: object?, a: A, next: Node?<A>) ensures Valid()
+    requires next != null ==> next.Valid() && next.owner == owner
+    ensures this.next == next
+    ensures this.value == a
+    ensures next != null ==> next.Repr == Repr - {this}
+    ensures this.owner == owner
+  {
+    this.value := a;
+    this.next := next;
+    this.Repr := if next == null then {this} else {this} + next.Repr;
+    this.size := if next == null then 1 else next.size + 1;
+    this.owner := owner;
+    new;
+  }
+
+  ghost predicate Valid()
+    reads this, Repr
+    decreases |Repr|
+  {
+    && 1 <= |Repr|
+    && this in Repr
+    && size == |Repr|
+    && (forall n: HasOwner <- Repr :: n.owner == owner)  // OWNER:
+    && (if next == null then Repr == {this}
+        else
+          && next in Repr
+          && next.Repr == Repr - {this}
+          && next.Valid())
+  }
+
+  function elemAt(index: nat): A
+    reads this, Repr
+    decreases |Repr|
+    requires Valid()
+    requires index < size
+  {
+    if index == 0 then value else next.elemAt(index - 1)
+  }
+
+  method replaceElemAt(index: nat, newElem: A)
+    modifies Repr
+    requires Valid()
+    ensures Repr == old(Repr)
+    ensures Valid()
+    ensures old(this.owner) == this.owner     // OWNER: 
+    requires index < size
+  {
+    if index == 0 {
+      this.value := newElem;
+    } else {
+      assert next == this || next.owner == this || next.owner == this.owner;      // OWNER (auto): 
+      next.replaceElemAt(index - 1, newElem);
+    }
+  }
+
+  method insertElemAt(index: nat, newElem: A)
+    returns (m: Node<A>, ghost insertedElem: Node<A>)
+    requires Valid()
+    requires index <= size
+    modifies Repr
+    ensures if index > 0 then m == this else m.next == this && m == insertedElem
+    ensures Valid()
+    ensures m.Valid()
+    ensures m.owner == this.owner                // OWNER: 
+    ensures m.size == old(size) + 1
+    ensures fresh(insertedElem)
+    ensures m.Repr == old(Repr) + {insertedElem}
+    ensures insertedElem.owner == this.owner
+  {
+    if index == 0 {
+      m := new Node<A>(this.owner, newElem, this); // OWNER: 
+      insertedElem := m;
+      return;
+    }
+    var newNext;
+    if index == 1 && next == null { // Insertion at the end
+      newNext := new Node<A>(this.owner, newElem, null);
+      insertedElem := newNext;
+    } else {
+      assert next == this || next.owner == this || next.owner == this.owner;     // OWNER (auto): 
+      newNext, insertedElem := next.insertElemAt(index - 1, newElem);
+    }
+    this.next := newNext;
+    Repr := {this} + newNext.Repr;
+    size := size + 1;
+    m := this;
+  }
+
+  method deleteElemAt(index: nat)
+    returns (m: Node?<A>, deleted: A)
+    requires Valid()
+    requires index < size
+    modifies Repr
+    ensures if old(size) > 1 then m != null && m.size == old(size - 1) else m == null
+    ensures deleted == old(elemAt(index))
+    ensures m != null ==>
+      && m.Repr < old(Repr)
+      && m.Valid()
+      && m.owner == this.owner   // OWNER: 
+  {
+    if index == 0 {
+      deleted := this.value;
+      m := this.next;
+      
+      assert if size > 1 then m != null && m.size == old(size - 1) else m == null;
+      assert m != null ==> m.Valid();
+      return;
+    }
+    assert next == this || next.owner == this || next.owner == this.owner;     // OWNER (auto): 
+    next, deleted := next.deleteElemAt(index - 1);
+    size := size - 1;
+    m := this;
+    assert next != null ==> this !in next.Repr;
+    Repr := if next == null then {this} else {this} + next.Repr;
+    assert next != null ==> next.Repr == Repr - {this};
+    assert if old(size) > 1 then m != null && m.size == old(size - 1) else m == null;
+    assert m != null ==> m.Valid();
+  }
+}
+
+
+
+
+
+
+
+
+
+
+
+
+
+
+
+
+
